change slice spec

main.c
@@ -2,11 +2,25 @@
 #include <stdio.h>
 #include "Slice.h"
 
+void print_sliced (uint32_t *u32_array, uint32_t u32_array_length, uint32_t from, uint32_t to) {
+  uint32_t *sliced = (uint32_t *)malloc(u32_array_length * sizeof(uint32_t));
+  uint32_t sliced_length = slice(u32_array, u32_array_length, sliced, from, to);
+  printf("[");
+  for(uint32_t i = 0; i < sliced_length; i ++) {
+    printf("%u", sliced[i]);
+    if (i != sliced_length - 1) {
+      printf(", ");
+    }
+  }
+  printf("]\n");
+  free(sliced);
+}
+
 int main() {
   uint32_t u32_array[] = {0, 1, 2, 3, 4};
   uint32_t u32_array_length = sizeof(u32_array) / sizeof(uint32_t);
-  struct_slice sliced = slice(u32_array, u32_array_length, 0, 5);
-  for(uint32_t i = 0; i < sliced.sliced_length; i ++) {
-    printf("%u\n", sliced.sliced[i]);
-  }
+  print_sliced(u32_array, u32_array_length, 0, 5);
+  print_sliced(u32_array, u32_array_length, 2, 4);
+  print_sliced(u32_array, u32_array_length, 5, 0);
+  return 0;
 }
