slice.fst
@@ -7,13 +7,6 @@ open LowStar.Printf
 module B = LowStar.Buffer
 module U32 = FStar.UInt32
 
-// #set-options "--z3rlimit 1000 --max_fuel 0 --max_ifuel 0 --detail_errors"
-
-noeq type struct_slice = {
-  sliced: B.buffer U32.t;
-  sliced_length: U32.t;
-}
-
 val slice_logic: 
   original: B.buffer U32.t ->
   original_length: U32.t ->
@@ -21,16 +14,14 @@ val slice_logic:
   sliced_length: U32.t ->
   from: U32.t ->
   to: U32.t ->
-  Stack (struct_slice) (requires fun h0 -> 
+  ST (sliced_length: U32.t) (requires fun h0 -> 
     B.live h0 original /\
     B.live h0 sliced /\
-    B.length original = U32.v original_length /\
-    B.length sliced = U32.v sliced_length 
+    B.length original = U32.v original_length /\ 
+    B.length sliced = U32.v original_length 
   )
   (ensures fun _ r h1 -> 
-  B.length r.sliced = U32.v r.sliced_length /\ 
-  (if (from = to) then U32.v sliced_length = U32.v r.sliced_length else true) /\
-  B.live h1 r.sliced
+    (if (from = to) then U32.v sliced_length = U32.v r else true)
   )
 let rec slice_logic original original_length sliced sliced_length from to =
   if U32.(
@@ -48,39 +39,26 @@ let rec slice_logic original original_length sliced sliced_length from to =
       slice_logic original original_length sliced sliced_length next_from_index to 
     )
   else if (from = to) then
-    {
-      sliced = sliced;
-      sliced_length = sliced_length;
-    }
+    sliced_length
   else
-    {
-      sliced = B.null;
-      sliced_length = 0ul;
-    }
+    0ul
 
 val slice:
   original: B.buffer U32.t ->
   original_length: U32.t ->
+  sliced: B.buffer U32.t ->
   from: U32.t ->
   to : U32.t ->
-  Stack (struct_slice) (requires fun h0 -> 
+  ST (sliced_length: U32.t) (requires fun h0 -> 
     B.live h0 original /\
-    B.length original = U32.v original_length
+    B.live h0 sliced /\
+    B.length original = U32.v original_length /\
+    B.length sliced = U32.v original_length
   )
-  (ensures fun h0 r h1 -> B.length r.sliced = U32.v r.sliced_length)
-let slice original original_length from to =
+  (ensures fun h0 r h1 -> true)
+let slice original original_length sliced from to =
   let sliced_length: U32.t = if U32.(from <^ to) then U32.(to -^ from) else 0ul in
   if (sliced_length = 0ul) then
-      {
-        sliced = B.null;
-        sliced_length = sliced_length;
-      }
+    0ul
   else
-    (
-      push_frame ();
-      let sliced: B.buffer U32.t = B.alloca 0ul sliced_length in
-      let sliced_struct: struct_slice = 
-        slice_logic original original_length sliced sliced_length from to in
-      pop_frame ();
-      sliced_struct
-    )
+    slice_logic original original_length sliced sliced_length from to
